extraction/theories/ESubstitution.v
@@ -2,7 +2,7 @@
 
 From Coq Require Import Bool String List Program BinPos Compare_dec Omega Lia.
 From Template Require Import config utils monad_utils BasicAst AstUtils.
-From PCUIC Require Import PCUICAst PCUICAstUtils PCUICInduction PCUICTyping PCUICWeakening PCUICSubstitution PCUICChecker PCUICRetyping PCUICMetaTheory PCUICWcbvEval PCUICSR PCUICValidity.
+From PCUIC Require Import PCUICAst PCUICAstUtils PCUICInduction PCUICTyping PCUICWeakening PCUICSubstitution PCUICChecker PCUICRetyping PCUICMetaTheory PCUICWcbvEval PCUICSR PCUICValidity PCUICWeakeningEnv.
 From TemplateExtraction Require Import EAst ELiftSubst ETyping EWcbvEval Extract Prelim.
 From Equations Require Import Equations.
 Require Import String.
@@ -14,36 +14,392 @@ Existing Instance config.default_checker_flags.
 Module PA := PCUICAst.
 Module P := PCUICWcbvEval.
 
-Inductive free : nat -> term -> Prop :=
-| free_tRel x : free x (tRel x)
-| free_tApp1 x s t : free x s -> free x (tApp s t)
-| free_tApp2 x s t : free x t -> free x (tApp s t)
-| free_tLambda x na s : free (S x) s -> free x (tLambda na s)
-| free_tProj x p s : free x s -> free x (tProj p s)
-| free_tFix x mfix n d : free (#|mfix| + x) (d.(dbody)) -> In d mfix -> free x (tFix mfix n)
-(* | free_tCoFix x m n : free x (tCoFix m n) *)
-| free_tCase1 x p s brs : free x s -> free x (tCase p s brs)
-| free_tCase2 x p s brs n b : free x b -> In (n, b) brs -> free x (tCase p s brs).
+Lemma All2_All_mix_left {A B} {P : A -> Type} {Q : A -> B -> Type}
+      {l : list A} {l'}:
+  All P l -> All2 Q l l' -> All2 (fun x y => (P x * Q x y)%type) l l'.
+Proof.
+  induction 2; simpl; intros; constructor.
+  inv X; intuition auto.
+  apply IHX0. inv X; intuition auto.
+Qed.
 
-Lemma subst_free_ext sigma tau t :
-  (forall n, free n t -> nth_error sigma n = nth_error tau n) -> subst sigma 0 t = subst tau 0 t.
-Admitted.
+(** ** Global Weakening  *)
+
+Lemma Is_type_extends Σ Γ t :
+  wf_local Σ Γ ->
+  forall Σ', wf Σ' -> extends Σ Σ' -> Is_Type_or_Proof Σ Γ t -> Is_Type_or_Proof Σ' Γ t.
+Proof.
+  intros. destruct X2 as [T []].
+  exists T. split. eapply weakening_env; [ | | eauto | | ]; eauto using wf_extends.
+  destruct s; eauto. 
+  destruct s as (u & ? & ?).
+  right. exists u. split; eauto.
+  eapply weakening_env; [ | | eauto | | ]; eauto using wf_extends.
+Qed.
+
+Lemma erases_extends :
+  env_prop (fun Σ Γ t T =>
+              forall Σ', wf Σ' -> extends Σ Σ' -> forall t', erases Σ Γ t t' -> erases Σ' Γ t t').
+Proof.
+  apply typing_ind_env; intros; rename_all_hyps.
+  all: match goal with [ H : erases _ _ ?a _ |- _ ] => tryif is_var a then idtac else inv H end.
+  all: try now (econstructor; eauto).  
+  all: try now (econstructor; eapply Is_type_extends; eauto).
+  - econstructor.  eauto. eapply All2_All_left in X3.
+    2:{ intros ? ? []. exact e. }
+    eapply All2_All_mix_left in H0; eauto.
+    eapply All2_impl. exact H0.
+    intros. destruct H3 as [? []].
+    split; eauto.
+  - econstructor.
+    eapply All2_All_mix_left in H; eauto.
+    eapply All2_impl. exact H.
+    intros ? ? [[[]] [? []]].
+    split; eauto.
+  - econstructor.
+    eapply All2_All_mix_left in H; eauto.
+    eapply All2_impl. exact H.
+    intros ? ? [[] [? []]].
+    split; eauto.
+  - eauto.
+Qed.
+
 
 (** ** Weakening *)
 
-Lemma erases_weakening (Σ : PCUICAst.global_context) (Γ Γ' : PCUICAst.context) (t T : PCUICAst.term) t' :
+Lemma Is_type_weakening:
+  forall (Σ : PCUICAst.global_context) (Γ Γ' Γ'' : PCUICAst.context),
+    wf_local Σ (Γ ,,, Γ') ->
+    wf Σ ->
+    wf_local Σ (Γ ,,, Γ'' ,,, lift_context #|Γ''| 0 Γ') ->
+    forall t : PCUICAst.term,
+      Is_Type_or_Proof Σ (Γ ,,, Γ') t -> Is_Type_or_Proof Σ (Γ ,,, Γ'' ,,, lift_context #|Γ''| 0 Γ') (PCUICLiftSubst.lift #|Γ''| #|Γ'| t).
+Proof.
+  intros. destruct X2 as (T & ? & ?).
+  eexists. split. eapply weakening_typing; eauto.
+  destruct s as [? | [u []]].
+  - left. clear - i. generalize (#|Γ''|), (#|Γ'|). induction T; cbn in *; intros; try now inv i.
+    + now eapply IHT2.
+    + now eapply IHT3.
+  - right. exists u. split; eauto.
+    eapply weakening_typing in t1; eauto.
+Qed.
+
+Lemma erases_weakening' (Σ : PCUICAst.global_context) (Γ Γ' Γ'' : PCUICAst.context) (t T : PCUICAst.term) t' :
     wf Σ ->
     wf_local Σ (Γ ,,, Γ') ->
-    Σ ;;; Γ |- t : T ->
-    Σ ;;; Γ |- t ⇝ℇ t' ->
-    Σ ;;; Γ ,,, Γ' |- (PCUICLiftSubst.lift #|Γ'| 0 t) ⇝ℇ (lift #|Γ'| 0 t').
+    wf_local Σ (Γ ,,, Γ'' ,,, lift_context #|Γ''| 0 Γ') -> 
+    Σ ;;; Γ ,,, Γ' |- t : T ->
+    Σ ;;; Γ ,,, Γ' |- t ⇝ℇ t' ->
+    Σ ;;; Γ ,,, Γ'' ,,, lift_context #|Γ''| 0 Γ' |- (PCUICLiftSubst.lift #|Γ''| #|Γ'| t) ⇝ℇ (lift #|Γ''| #|Γ'| t').
 Proof.
+  intros HΣ HΓΓ' HΓ'' * H He.
+  generalize_eqs H. intros eqw. rewrite <- eqw in *.
+  revert Γ Γ' Γ'' HΓ'' eqw t' He.
+  revert Σ HΣ Γ0 HΓΓ' t T H .
+  apply (typing_ind_env (fun Σ Γ0 t T =>  forall Γ Γ' Γ'',
+    wf_local Σ (Γ ,,, Γ'' ,,, lift_context #|Γ''| 0 Γ') ->
+    Γ0 = Γ ,,, Γ' ->
+    forall t',
+    Σ;;; Γ0 |- t ⇝ℇ t' ->
+    _));
+    intros Σ wfΣ Γ0; !!intros; subst Γ0.
+  all: match goal with [ H : erases _ _ ?a _ |- _ ] => tryif is_var a then idtac else inv H end.
+  all: try now (cbn; econstructor; eauto).
+  all: try now (econstructor; eapply Is_type_weakening; eauto).
+  all:cbn.
+  - destruct ?; econstructor. 
+  - econstructor.
+    unfold app_context, PCUICAst.snoc in *.    
+    pose proof (h_forall_Γ0 (Γ) (PCUICAst.vass n t :: Γ') Γ'').
+    rewrite lift_context_snoc0, <- plus_n_O in *.
+    eapply H0; eauto. cbn. econstructor.
+    eauto. cbn. exists s1. eapply weakening_typing with (T := tSort s1); eauto.
+  - econstructor.
+    + eapply h_forall_Γ0; eauto.
+    + pose proof (h_forall_Γ1 Γ (PCUICAst.vdef n b b_ty :: Γ') Γ'').
+      rewrite lift_context_snoc0, <- plus_n_O in *.
+      eapply H1; eauto. cbn. econstructor.
+      eauto. cbn. eapply weakening_typing; eauto.
+  - econstructor.
+    + eapply h_forall_Γ0; eauto.
+    + eapply All2_map.
+      eapply All2_All_left in X3.
+      2:{ intros. destruct X1. exact e. }
+      eapply All2_impl. eapply All2_All_mix_left.
+      eassumption. eassumption. intros.
+      destruct H3. destruct p0.
+      cbn. destruct x, y; cbn in *; subst.
+      split; eauto.
+  - econstructor.
+    eapply All2_map.
+    eapply All2_impl. eapply All2_All_mix_left.
+    eassumption. eassumption. intros.
+    destruct X1 as [[[]] [? []]].
+    destruct x, y; cbn in *; subst.
+    repeat split. unfold app_context in *.
+    eapply (e0 Γ (types ++ Γ') Γ'') in e3.
+    3: now rewrite app_assoc. 
+    2:rewrite lift_context_app.
+    2:{ admit. (* wf_local *) }
+    rewrite app_length in *.
+    subst types. rewrite fix_context_length in *.
+    rewrite (All2_length _ _ H) in *.
+    Lemma erases_ctx_ext Σ Γ Γ' t t' :
+      erases Σ Γ t t' -> Γ = Γ' -> erases Σ Γ' t t'.
+    Proof.
+      intros. now subst.
+    Qed.
+    eapply erases_ctx_ext. eapply e3.
+    rewrite lift_context_app. unfold app_context.
+    rewrite !app_assoc. repeat f_equal.
+    rewrite <- lift_fix_context.
+    rewrite <- plus_n_O.
+    now rewrite (All2_length _ _ H).
+  - econstructor.
+    eapply All2_map.
+    eapply All2_impl. eapply All2_All_mix_left.
+    eassumption. eassumption. intros.
+    destruct X1 as [[] [? []]].
+    destruct x, y; cbn in *; subst.
+    repeat split. unfold app_context in *.
+    eapply (e Γ (types ++ Γ') Γ'') in e2.
+    3: now rewrite app_assoc. 
+    2:rewrite lift_context_app.
+    2: admit. (* wf_local *)
+    rewrite app_length in *.
+    subst types. rewrite fix_context_length in *.
+    rewrite (All2_length _ _ H) in *.
+    eapply erases_ctx_ext. eapply e2.
+    rewrite lift_context_app. unfold app_context.
+    rewrite !app_assoc. repeat f_equal.
+    rewrite <- lift_fix_context.
+    rewrite <- plus_n_O.
+    now rewrite (All2_length _ _ H).
 Admitted.
+
+Lemma erases_weakening (Σ : PCUICAst.global_context) (Γ Γ' : PCUICAst.context) (t T : PCUICAst.term) t' :
+  wf Σ ->
+  wf_local Σ (Γ ,,, Γ') ->
+  Σ ;;; Γ |- t : T ->
+  Σ ;;; Γ |- t ⇝ℇ t' ->
+  Σ ;;; Γ ,,, Γ' |- (PCUICLiftSubst.lift #|Γ'| 0 t) ⇝ℇ (lift #|Γ'| 0 t').
+Proof.
+  intros.
+  pose proof (typing_wf_local X1).
+  eapply (erases_weakening' Σ Γ [] Γ'); cbn; eauto.
+Qed.  
+
+Lemma All2_nth_error_None {A B} {P : A -> B -> Type} {l l'} n :
+  All2 P l l' ->
+  nth_error l n = None ->
+  nth_error l' n = None.
+Proof.
+  intros Hall. revert n.
+  induction Hall; destruct n; simpl; try congruence. auto.
+Qed.
+
+Lemma All2_length {A B} {P : A -> B -> Type} l l' : All2 P l l' -> #|l| = #|l'|.
+Proof. induction 1; simpl; auto. Qed.
+
+Lemma is_type_subst Σ Γ Γ' Δ a s :
+  wf Σ -> subslet Σ Γ s Γ' ->
+  (* Σ ;;; Γ ,,, Γ' ,,, Δ |- a : T -> *)
+  wf_local Σ (Γ ,,, subst_context s 0 Δ) ->
+  Is_Type_or_Proof Σ (Γ ,,, Γ' ,,, Δ) a ->
+  Is_Type_or_Proof Σ (Γ ,,, subst_context s 0 Δ) (PCUICLiftSubst.subst s #|Δ| a).
+Proof.
+  intros ? ? ? (T & HT & H).
+  exists (PCUICLiftSubst.subst s #|Δ| T). split.
+  eapply substitution; eauto.
+  destruct H as [ | (u & ? & ?) ].
+  - left. generalize (#|Δ|). intros n.
+    induction T in n, i |- *; (try now inv i); cbn in *; eauto.
+  - right. exists u. split; eauto.
+    pose proof (substitution Σ Γ Γ' s Δ).
+    eapply X2 in t; eauto.
+Qed.
+
+Lemma erases_subst Σ Γ Γ' Δ t s t' s' T :
+  wf Σ ->
+  subslet Σ Γ s Γ' ->
+  wf_local Σ (Γ ,,, subst_context s 0 Δ) ->
+  Σ ;;; Γ ,,, Γ'  ,,, Δ |- t : T ->
+  Σ ;;; Γ ,,, Γ'  ,,, Δ |- t ⇝ℇ t' ->                            
+  All2 (erases Σ Γ) s s' ->
+  Σ ;;; (Γ ,,, subst_context s 0 Δ) |- (PCUICLiftSubst.subst s #|Δ| t) ⇝ℇ subst s' #|Δ| t'.
+Proof.
+  intros HΣ HΔ Hs Ht He.
+  pose proof (typing_wf_local Ht).
+  generalize_eqs Ht. intros eqw. rewrite <- eqw in X.
+  revert Γ Γ' Δ t' s Hs HΔ He eqw.
+  revert Σ HΣ Γ0 X t T Ht.
+  eapply (typing_ind_env (fun Σ Γ0 t T =>
+                            forall (Γ Γ' : PCUICAst.context) Δ t' (s : list PCUICAst.term),
+                              wf_local Σ (Γ ,,, subst_context s 0 Δ) ->
+                              subslet Σ Γ s Γ' ->
+                              Σ;;; Γ ,,, Γ' ,,, Δ |- t ⇝ℇ t' ->
+                              Γ0 = Γ ,,, Γ' ,,, Δ ->
+                              All2 (erases Σ Γ) s s' ->
+                              Σ;;; Γ ,,, subst_context s 0 Δ |- PCUICLiftSubst.subst s #|Δ| t ⇝ℇ subst s' #|Δ| t'
+         ));
+    intros Σ wfΣ Γ0 wfΓ0; intros; simpl in * |-; subst Γ0.
+  - inv H0.
+    + cbn. destruct ?. destruct ?.
+      * eapply All2_nth_error_Some in H2; eauto.
+        destruct H2 as (? & ? & ?).
+        rewrite e.
+        erewrite <- subst_context_length.
+        eapply erases_weakening; eauto.
+        (* subslet and typing *) admit.
+      * erewrite All2_length; eauto.                
+        eapply All2_nth_error_None in H2; eauto.
+        rewrite H2. econstructor.
+      * econstructor.
+    + econstructor.
+      eapply is_type_subst; eauto.
+  - inv H. econstructor.
+    eapply is_type_subst; eauto.
+  - inv H1. econstructor.
+    eapply is_type_subst; eauto.
+  - inv H1.
+    + cbn. econstructor.
+      specialize (H0 Γ Γ' (PCUICAst.vass n t :: Δ) t'0 s).
+      (* unfold app_context, snoc in *. *)
+      rewrite subst_context_snoc0 in *.
+      eapply H0; eauto.
+      cbn. econstructor. eauto.
+      cbn. exists s1. eapply substitution with (T := tSort s1); eauto.
+    + econstructor.
+      eapply is_type_subst; eauto.
+  - inv H2.
+    + cbn. econstructor.
+      eauto.
+      specialize (H1 Γ Γ' (PCUICAst.vdef n b b_ty :: Δ) t2' s).
+      rewrite subst_context_snoc0 in *.
+      eapply H1; eauto.
+      cbn. econstructor. eauto.
+      cbn. eapply substitution; eauto.
+    + econstructor.
+      eapply is_type_subst; eauto.
+  - inv H1.
+    + cbn. econstructor.
+      eapply H; eauto.
+      eapply H0; eauto.
+    + econstructor.
+      eapply is_type_subst; eauto.
+  - inv H1.
+    + cbn. econstructor.
+    + econstructor.
+      eapply is_type_subst; eauto.
+  - inv H0. econstructor.
+    eapply is_type_subst; eauto.
+  - inv H0.
+    + cbn. econstructor. 
+    + econstructor.
+      eapply is_type_subst; eauto.
+  - depelim H5. 
+    + cbn. econstructor.
+      eapply H4; eauto.
+      eapply All2_map.
+      eapply All2_impl_In; eauto.
+      intros. destruct H10, x, y. cbn in *. subst. split; eauto.
+      eapply All2_All_left in X3.
+      2:{ intros ? ? []. exact e0. }
+
+      eapply In_nth_error in H8 as [].
+      eapply nth_error_all in X3; eauto.
+      eapply X3; eauto.      
+    (* + cbn. econstructor. *)
+    (*   eapply H4 in H5; eauto. *)
+    (*   econstructor. *)
+    (* + cbn.  *)
+
+    (*   Lemma subst_mkppBox s m n x : *)
+    (*     subst s m (mkAppBox x n) = mkAppBox (subst s m x) n. *)
+    (*   Proof. *)
+    (*     revert x; induction n; cbn; intros; try congruence. *)
+    (*     now rewrite IHn. *)
+    (*   Qed. *)
+    (*   rewrite subst_mkppBox. *)
+    (*   econstructor. *)
+    (*   eapply H4 in H5_; eauto. *)
+    (*   inv X3. destruct X6. *)
+    (*   eapply e; eauto. *)
+    + econstructor.
+      eapply is_type_subst; eauto.      
+  - inv H1.
+    + cbn. econstructor.
+      eauto.
+    + econstructor.
+      eapply is_type_subst; eauto.
+  - inv H0.
+    + cbn. econstructor.
+      eapply All2_map.
+      eapply All2_impl_In.
+      eassumption.
+      intros. destruct H4 as (? & ? & ?).
+      repeat split; eauto.
+      eapply In_nth_error in H0 as [].
+      eapply nth_error_all in X0; eauto.
+      destruct X0.
+      specialize (e2 Γ Γ' (Δ ,,, PCUICLiftSubst.fix_context mfix)).
+      rewrite app_context_assoc in *.
+      eapply e2 in e1; eauto.
+
+      Lemma erases_eq Σ Γ Γ' t t' s s' :
+        erases Σ Γ t t' -> 
+        Γ = Γ' ->
+        t = s ->
+        t' = s' ->      
+        erases Σ Γ' s s'.
+      Proof.
+        now subst.
+      Qed.
+      eapply erases_eq; eauto.
+      * rewrite subst_context_app.
+        rewrite <- plus_n_O.
+        rewrite app_context_assoc. f_equal.
+        now rewrite subst_fix_context.
+      * cbn. now rewrite app_context_length, fix_context_length.
+      * cbn. now erewrite app_context_length, fix_context_length, All2_length.
+      * admit. (* wf_local *)
+    + econstructor.
+      eapply is_type_subst; eauto.
+  -  inv H0.
+    + cbn. econstructor.
+      eapply All2_map.
+      eapply All2_impl_In.
+      eassumption.
+      intros. destruct H4 as (? & ? & ?).
+      repeat split; eauto.
+      eapply In_nth_error in H0 as [].
+      eapply nth_error_all in X0; eauto.
+      destruct X0.
+      specialize (e2 Γ Γ' (Δ ,,, PCUICLiftSubst.fix_context mfix)).
+      rewrite app_context_assoc in *.
+      eapply e2 in e1; eauto.
+
+      eapply erases_eq; eauto.
+      * rewrite subst_context_app.
+        rewrite <- plus_n_O.
+        rewrite app_context_assoc. f_equal.
+        now rewrite subst_fix_context.
+      * cbn. now rewrite app_context_length, fix_context_length.
+      * cbn. now erewrite app_context_length, fix_context_length, All2_length.
+      * admit. (* wf_local *)
+    + econstructor.
+      eapply is_type_subst; eauto.
+  - eapply H; eauto.    
+Admitted.  
 
 (* Lemma extract_weakening (Σ : PCUICAst.global_context) (Γ Γ' : PCUICAst.context) (t T : PCUICAst.term) : *)
 (*     wf Σ -> *)
 (*     wf_local Σ (Γ ,,, Γ') -> *)
 (*     Σ;;; Γ |- t : T -> *)
+(*      Σ ;;; Γ |- t ⇝ℇ t' -> *)
+(*     Σ ;;; Γ ,,, Γ'' ,,, lift_context #|Γ''| 0 Γ' |- (PCUICLiftSubst.lift #|Γ''| #|Γ'| t) ⇝ℇ (lift #|Γ''| #|Γ'| t'). *)
+                 
 (*     extract Σ (Γ ,,, Γ') (PCUICLiftSubst.lift #|Γ'| 0 t) = lift #|Γ'| 0 (extract Σ Γ t). *)
 (* Proof. *)
 (* Admitted. *)
@@ -139,29 +495,10 @@ Admitted.
 (*   - apply IHX. *)
 (* Qed. *)
 
-Lemma bool_equiv b1 b2 T1 T2 : 
-(b1 = true <~> T1) -> (b2 = true <~> T2) -> T1 <~> T2 -> b1 = b2.
-Proof.
-Admitted.
-
-Lemma is_type_subst Σ Γ Γ' Δ a s :
-  wf Σ -> subslet Σ Γ s Γ' ->
-  (* Σ ;;; Γ ,,, Γ' ,,, Δ |- a : T -> *)
-  wf_local Σ (Γ ,,, subst_context s 0 Δ) ->
-  Is_Type_or_Proof Σ (Γ ,,, Γ' ,,, Δ) a ->
-  Is_Type_or_Proof Σ (Γ ,,, subst_context s 0 Δ) (PCUICLiftSubst.subst s #|Δ| a).
-Proof.
-  intros ? ? ? (T & HT & H).
-  exists (PCUICLiftSubst.subst s #|Δ| T). split.
-  eapply substitution; eauto.
-  destruct H as [ | (u & ? & ?) ].
-  - left. generalize (#|Δ|). intros n.
-    induction T in n, i |- *; (try now inv i); cbn in *; eauto.
-  - right. exists u. split; eauto.
-    pose proof (substitution Σ Γ Γ' s Δ).
-    eapply X2 in t; eauto.
-Qed.
-
+(* Lemma bool_equiv b1 b2 T1 T2 :  *)
+(* (b1 = true <~> T1) -> (b2 = true <~> T2) -> T1 <~> T2 -> b1 = b2. *)
+(* Proof. *)
+(* Admitted. *)
 
 (* Lemma is_type_subst Σ Γ Γ' Δ a T s : *)
 (*   wf Σ -> subslet Σ Γ s Γ' -> *)
@@ -198,202 +535,7 @@ Qed.
 (*       * right. exists u. split; eauto. *)
 (* Qed. *)
 
-Lemma All2_nth_error_None {A B} {P : A -> B -> Type} {l l'} n :
-  All2 P l l' ->
-  nth_error l n = None ->
-  nth_error l' n = None.
-Proof.
-  intros Hall. revert n.
-  induction Hall; destruct n; simpl; try congruence. auto.
-Qed.
-Lemma All2_length {A B} {P : A -> B -> Type} l l' : All2 P l l' -> #|l| = #|l'|.
-Proof. induction 1; simpl; auto. Qed.
 
-
-Lemma erases_subst Σ Γ Γ' Δ t s t' s' T :
-  wf Σ ->
-  subslet Σ Γ s Γ' ->
-  wf_local Σ (Γ ,,, subst_context s 0 Δ) ->
-  Σ ;;; Γ ,,, Γ'  ,,, Δ |- t : T ->
-  Σ ;;; Γ ,,, Γ'  ,,, Δ |- t ⇝ℇ t' ->                            
-  All2 (erases Σ Γ) s s' ->
-  Σ ;;; (Γ ,,, subst_context s 0 Δ) |- (PCUICLiftSubst.subst s #|Δ| t) ⇝ℇ subst s' #|Δ| t'.
-Proof.
-  intros HΣ HΔ Hs Ht He.
-  pose proof (typing_wf_local Ht).
-  generalize_eqs Ht. intros eqw. rewrite <- eqw in X.
-  revert Γ Γ' Δ t' s Hs HΔ He eqw.
-  revert Σ HΣ Γ0 X t T Ht.
-  eapply (typing_ind_env (fun Σ Γ0 t T =>
-                            forall (Γ Γ' : PCUICAst.context) Δ t' (s : list PCUICAst.term),
-                              wf_local Σ (Γ ,,, subst_context s 0 Δ) ->
-                              subslet Σ Γ s Γ' ->
-                              Σ;;; Γ ,,, Γ' ,,, Δ |- t ⇝ℇ t' ->
-                              Γ0 = Γ ,,, Γ' ,,, Δ ->
-                              All2 (erases Σ Γ) s s' ->
-                              Σ;;; Γ ,,, subst_context s 0 Δ |- PCUICLiftSubst.subst s #|Δ| t ⇝ℇ subst s' #|Δ| t'
-         ));
-    intros Σ wfΣ Γ0 wfΓ0; intros; simpl in * |-; subst Γ0.
-  - inv H0.
-    + cbn. destruct ?. destruct ?.
-      * eapply All2_nth_error_Some in H2; eauto.
-        destruct H2 as (? & ? & ?).
-        rewrite e.
-        erewrite <- subst_context_length.
-        eapply erases_weakening; eauto.
-        (* subslet and typing *) admit.
-      * erewrite All2_length; eauto.                
-        eapply All2_nth_error_None in H2; eauto.
-        rewrite H2. econstructor.
-      * econstructor.
-    + econstructor.
-      eapply substitution; eauto.
-      eapply is_type_subst; eauto.
-  - inv H. econstructor.
-    eapply substitution; eauto.
-    eapply is_type_subst; eauto.
-  - inv H1. econstructor.
-    eapply substitution; eauto.
-    eapply is_type_subst; eauto.
-  - inv H1.
-    + cbn. econstructor.
-      specialize (H0 Γ Γ' (PCUICAst.vass n t :: Δ) t'0 s).
-      (* unfold app_context, snoc in *. *)
-      rewrite subst_context_snoc0 in *.
-      eapply H0; eauto.
-      admit. (* wf_local *)
-    + econstructor.
-      eapply substitution; eauto.
-      eapply is_type_subst; eauto.
-  - inv H2.
-    + cbn. econstructor.
-      eauto.
-      specialize (H1 Γ Γ' (PCUICAst.vdef n b b_ty :: Δ) t2' s).
-      rewrite subst_context_snoc0 in *.
-      eapply H1; eauto.
-      admit. (* wf_local *)
-    + econstructor.
-      eapply substitution; eauto.
-      eapply is_type_subst; eauto.
-  - inv H1.
-    + cbn. econstructor.
-      eapply H; eauto.
-      eapply H0; eauto.
-    + econstructor.
-      eapply substitution; eauto.
-      eapply is_type_subst; eauto.
-  - inv H1.
-    + cbn. econstructor.
-    + econstructor.
-      eapply substitution; eauto.
-      eapply is_type_subst; eauto.
-  - inv H0. econstructor.
-    eapply substitution; eauto.
-    eapply is_type_subst; eauto.
-  - inv H0.
-    + cbn. econstructor. 
-    + econstructor.
-      eapply substitution; eauto.
-      eapply is_type_subst; eauto.
-  - depelim H5. 
-    + cbn. econstructor.
-      eapply H4; eauto.
-      eapply All2_map.
-      eapply All2_impl_In; eauto.
-      intros. destruct H10, x, y. cbn in *. subst. split; eauto.
-      eapply All2_All_left in X3.
-      2:{ intros ? ? []. exact e0. }
-
-      eapply In_nth_error in H8 as [].
-      eapply nth_error_all in X3; eauto.
-      eapply X3; eauto.      
-    + cbn. econstructor.
-      eapply H4 in H5; eauto.
-      econstructor.
-    + cbn. 
-
-      Lemma subst_mkppBox s m n x :
-        subst s m (mkAppBox x n) = mkAppBox (subst s m x) n.
-      Proof.
-        revert x; induction n; cbn; intros; try congruence.
-        now rewrite IHn.
-      Qed.
-      rewrite subst_mkppBox.
-      econstructor.
-      eapply H4 in H5_; eauto.
-      inv X3. destruct X6.
-      eapply e; eauto.
-    + econstructor.
-      eapply substitution; eauto.
-      eapply is_type_subst; eauto.      
-  - inv H1.
-    + cbn. econstructor.
-      eauto.
-    + econstructor.
-      eapply substitution; eauto.
-      eapply is_type_subst; eauto.
-  - inv H0.
-    + cbn. econstructor.
-      eapply All2_map.
-      eapply All2_impl_In.
-      eassumption.
-      intros. destruct H4 as (? & ? & ?).
-      repeat split; eauto.
-      eapply In_nth_error in H0 as [].
-      eapply nth_error_all in X0; eauto.
-      destruct X0.
-      specialize (e2 Γ Γ' (Δ ,,, PCUICLiftSubst.fix_context mfix)).
-      rewrite app_context_assoc in *.
-      eapply e2 in e1; eauto.
-
-      Lemma erases_eq Σ Γ Γ' t t' s s' :
-        erases Σ Γ t t' -> 
-        Γ = Γ' ->
-        t = s ->
-        t' = s' ->      
-        erases Σ Γ' s s'.
-      Proof.
-        now subst.
-      Qed.
-      eapply erases_eq; eauto.
-      * rewrite subst_context_app.
-        rewrite <- plus_n_O.
-        rewrite app_context_assoc. f_equal.
-        now rewrite subst_fix_context.
-      * cbn. now rewrite app_context_length, fix_context_length.
-      * cbn. now erewrite app_context_length, fix_context_length, All2_length.
-      * admit. (* wf_local *)
-    + econstructor.
-      eapply substitution; eauto.
-      eapply is_type_subst; eauto.
-  -  inv H0.
-    + cbn. econstructor.
-      eapply All2_map.
-      eapply All2_impl_In.
-      eassumption.
-      intros. destruct H4 as (? & ? & ?).
-      repeat split; eauto.
-      eapply In_nth_error in H0 as [].
-      eapply nth_error_all in X0; eauto.
-      destruct X0.
-      specialize (e2 Γ Γ' (Δ ,,, PCUICLiftSubst.fix_context mfix)).
-      rewrite app_context_assoc in *.
-      eapply e2 in e1; eauto.
-
-      eapply erases_eq; eauto.
-      * rewrite subst_context_app.
-        rewrite <- plus_n_O.
-        rewrite app_context_assoc. f_equal.
-        now rewrite subst_fix_context.
-      * cbn. now rewrite app_context_length, fix_context_length.
-      * cbn. now erewrite app_context_length, fix_context_length, All2_length.
-      * admit. (* wf_local *)
-    + econstructor.
-      eapply substitution; eauto.
-      eapply is_type_subst; eauto.
-  - eapply H; eauto.    
-Admitted.  
-  
   (* ============================ *)
   (* forall Σ : PCUICAst.global_context, *)
   (* wf Σ -> *)
